tests/list/expected.tst
@@ -3,5 +3,4 @@ data list (A : ★) : ★ =
   | nil : list
   | cons : A ➔ list ➔ list.
 
-_ = list.
 
