tests/nat/expected.tst
@@ -3,5 +3,4 @@ data nat : ★ =
   | O : nat
   | S : nat ➔ nat.
 
-_ = nat.
 
