tests/option/expected.tst
@@ -3,5 +3,4 @@ data option (A : ★) : ★ =
   | Some : A ➔ option
   | None : option.
 
-_ = option.
 
