tests/vector/expected.tst
@@ -7,5 +7,4 @@ data t (A : ★) : nat ➔ ★ =
   | nil : t O
   | cons : Π h : A . Π n : nat . t n ➔ t (S n).
 
-_ = t.
 
